update Domain

Lambda/Domain.lean
@@ -5,24 +5,27 @@ import Mathlib.Order.Monotone.Basic
 import Mathlib.Order.Bounds.Basic
 import Mathlib.Tactic.ApplyAt
 
-namespace Domain
-
-lemma Monotone.prod_fst [PartialOrder α] [PartialOrder β] :
-  Monotone (Prod.fst : α × β → α) := λ _ _ => And.left
-
-lemma Monotone.prod_snd [PartialOrder α] [PartialOrder β] :
-  Monotone (Prod.snd : α × β → β) := λ _ _ => And.right
-
-
-
-def Directed [PartialOrder α] (s : Set α) : Prop :=
-  s.Nonempty ∧ ∀ x ∈ s, ∀ y ∈ s, ∃ z ∈ s, x ≤ z ∧ y ≤ z
-
-namespace Directed
+namespace Monotone
 
 variable [PartialOrder α] [PartialOrder β]
 
-theorem singleton {x : α} : Directed {x} := by
+lemma prod_fst : Monotone (Prod.fst : α × β → α) :=
+  λ _ _ => And.left
+
+lemma prod_snd : Monotone (Prod.snd : α × β → β) :=
+  λ _ _ => And.right
+
+end Monotone
+
+
+def Directed' [PartialOrder α] (s : Set α) : Prop :=
+  s.Nonempty ∧ ∀ x ∈ s, ∀ y ∈ s, ∃ z ∈ s, x ≤ z ∧ y ≤ z
+
+namespace Directed'
+
+variable [PartialOrder α] [PartialOrder β]
+
+theorem singleton {x : α} : Directed' {x} := by
   constructor
   · exists x
   · intros _ h₁ _ h₂
@@ -30,7 +33,7 @@ theorem singleton {x : α} : Directed {x} := by
     exists x
 
 theorem prod {s : Set α} {t : Set β}
-  (hs : Directed s) (ht : Directed t) : Directed (s ×ˢ t) := by
+  (hs : Directed' s) (ht : Directed' t) : Directed' (s ×ˢ t) := by
   constructor
   · rcases hs.1 with ⟨x, h₁⟩
     rcases ht.1 with ⟨y, h₂⟩
@@ -41,7 +44,7 @@ theorem prod {s : Set α} {t : Set β}
     exists ⟨z₁, z₂⟩
 
 theorem mono_image {f : α → β} {s : Set α}
-  (hs : Directed s) (hf : Monotone f) : Directed (f '' s) := by
+  (hs : Directed' s) (hf : Monotone f) : Directed' (f '' s) := by
   constructor
   · rcases hs.1 with ⟨x, h⟩
     exists f x, x
@@ -51,21 +54,21 @@ theorem mono_image {f : α → β} {s : Set α}
     exists f z, ⟨z, ?_⟩ <;> aesop
 
 theorem prod_fst {s : Set (α × β)}
-  (hs : Directed s) : Directed (Prod.fst '' s) :=
+  (hs : Directed' s) : Directed' (Prod.fst '' s) :=
   mono_image hs Monotone.prod_fst
 
 theorem prod_snd {s : Set (α × β)}
-  (hs : Directed s) : Directed (Prod.snd '' s) :=
+  (hs : Directed' s) : Directed' (Prod.snd '' s) :=
   mono_image hs Monotone.prod_snd
 
 theorem mono_range {f : α → β}
-  (hs : Directed (Set.univ : Set α)) (hf : Monotone f) :
-  Directed (Set.range f) := by
+  (hs : Directed' (Set.univ : Set α)) (hf : Monotone f) :
+  Directed' (Set.range f) := by
   rw [←Set.image_univ]
   exact mono_image hs hf
 
 theorem mono_comp_image {f : α → β} {s : Set ι} {g : ι → α}
-  (hg : Directed (g '' s)) (hf : Monotone f) : Directed ((f ∘ g) '' s) := by
+  (hg : Directed' (g '' s)) (hf : Monotone f) : Directed' ((f ∘ g) '' s) := by
   constructor
   · rcases hg.1 with ⟨_, ⟨x, h, h'⟩⟩
     subst h'
@@ -76,15 +79,15 @@ theorem mono_comp_image {f : α → β} {s : Set ι} {g : ι → α}
     exists f (g z)
     aesop
 
-theorem mono_comp_range {ι : Type w} {f : α → β} {g : ι → α}
-  (hg : Directed (Set.range g)) (hf : Monotone f) : Directed (Set.range (f ∘ g)) := by
+theorem mono_comp_range {ι : Type u} {f : α → β} {g : ι → α}
+  (hg : Directed' (Set.range g)) (hf : Monotone f) : Directed' (Set.range (f ∘ g)) := by
   rw [←Set.image_univ] at *
   exact mono_comp_image hg hf
 
-end Directed
+end Directed'
 
-theorem Directed.linear_order [LinearOrder α] {s : Set α}
-  (h : s.Nonempty) : Directed s := by
+theorem Directed'.linear_order [LinearOrder α] {s : Set α}
+  (h : s.Nonempty) : Directed' s := by
   constructor
   · exact h
   · intros x h₁ y h₂
@@ -92,14 +95,14 @@ theorem Directed.linear_order [LinearOrder α] {s : Set α}
     · exists y
     · exists x
 
-theorem Directed.linear_order_univ [LinearOrder α] [Nonempty α] :
-  Directed (Set.univ : Set α) :=
-  Directed.linear_order Set.univ_nonempty
+theorem Directed'.linear_order_univ [LinearOrder α] [Nonempty α] :
+  Directed' (Set.univ : Set α) :=
+  Directed'.linear_order Set.univ_nonempty
 
 
 
 class Dcpo (α : Type u) extends PartialOrder α where
-  sSup : ∀ (s : Set α), Directed s → α
+  sSup : ∀ (s : Set α), Directed' s → α
   sSup_is_lub : ∀ s hs, IsLUB s (@sSup s hs)
 
 namespace Dcpo
@@ -116,7 +119,7 @@ theorem sSup_le {s : Set α} {hs} : (∀ y ∈ s, y ≤ x) → sSup s hs ≤ x :
   apply (Dcpo.sSup_is_lub s _).right
   exact h
 
-def iSup (f : ι → α) (hf : Directed (Set.range f)) :=
+def iSup (f : ι → α) (hf : Directed' (Set.range f)) :=
   sSup (Set.range f) hf
 
 theorem iSup.sSup {f : ι → α} {hf} : sSup (Set.range f) hf = iSup f hf := rfl
@@ -133,7 +136,15 @@ theorem iSup_le {f : ι → α} {hf} :
   subst h'
   apply h
 
-def iSupMem (s : Set ι) (f : ι → α) (hf : Directed (f '' s)) :=
+theorem iSup.mono {f g : ι → α} {hf hg} :
+  (∀ i, f i ≤ g i) → iSup f hf ≤ iSup g hg := by
+  intro h
+  apply iSup_le
+  intro i
+  apply le_trans (h i)
+  exact le_iSup
+
+def iSupMem (s : Set ι) (f : ι → α) (hf : Directed' (f '' s)) :=
   sSup (f '' s) hf
 
 theorem iSupMem.sSup {f : ι → α} {hf} : sSup (f '' s) hf = iSupMem s f hf := rfl
@@ -159,150 +170,42 @@ theorem iSupMem.comp {s : Set ι} {f : α → β} {g : ι → α} {hf} {hfg} :
   congr
   rw [Set.image_comp]
 
-instance : Dcpo PUnit where
-  sSup := λ s _ => ()
-  sSup_is_lub := by
-    intros _ _; constructor <;> intros _ _ <;> trivial
+theorem iSupMem.mono {s : Set ι} {f g : ι → α} {hf} {hg} :
+  (∀ i ∈ s, f i ≤ g i) → iSupMem s f hf ≤ iSupMem s g hg := by
+  intro h
+  apply iSupMem_le
+  intros i h'
+  apply le_trans (h i h')
+  exact le_iSupMem h'
 
-noncomputable def flat (α : Type u) : Dcpo α where
-  le := λ x y => x = y
-  le_refl := by intro; simp
-  le_trans := by intros _ _ _ h₁ h₂; simp at *; simp [h₁, h₂]
-  le_antisymm := by intros _ _ h₁ _; simp at *; exact h₁
-  sSup := λ s hs => Classical.choose (by cases' hs with hs; exact hs)
-  sSup_is_lub := by
-    intro s hs
-    cases' hs with hs₁ hs₂
-    have h : ∀ x (_ : x ∈ s) (h' : s.Nonempty), Classical.choose h' = x := by
-      intros x h h'
-      let y := Classical.choose h'
-      rcases hs₂ x h y (Classical.choose_spec h') with ⟨z, _, h₃, h₄⟩
-      simp at *
-      simp [h₃, h₄]
-    constructor
-    · intros y h₁
-      simp [h y h₁]
-    · cases' hs₁ with x h₁
-      intros y h₂
-      have h₃ := h₂ h₁
-      simp at h₃
-      simp [←h₃, h x h₁]
-
-noncomputable instance lift : Dcpo (WithBot α) where
-  sSup := λ s hs =>
-    have := Classical.propDecidable
-    if h : ∃ x, some x ∈ s then
-      @Dcpo.sSup α _ { x | some x ∈ s } (by
-        constructor
-        · rcases h with ⟨x, h⟩
-          exists x
-        · intro x h₁ y h₂
-          rcases hs.2 _ h₁ _ h₂ with ⟨z, h₃, h₄, h₅⟩
-          cases' z with z
-          · apply le_bot_iff.1 at h₄
-            contradiction
-          · simp at h₄ h₅
-            exists z)
-    else ⊥
-  sSup_is_lub := by
-    intros s hs
-    by_cases h : ∃ x, some x ∈ s <;> simp [h]
-    · constructor
-      · intros x h₁ y h₂
-        simp at h₂
-        subst h₂
-        refine ⟨_, rfl, ?_⟩
-        apply le_sSup
-        exact h₁
-      · intros x h₁
-        cases' x with x
-        · cases' h with y h
-          have h₂ := h₁ h
-          apply le_bot_iff.1 at h₂
-          contradiction
-        · apply WithBot.some_le_some.2
-          apply sSup_le
-          intro y h₂
-          apply h₁ at h₂
-          simp at h₂
-          exact h₂
-    · constructor
-      · intros x h₁ y h₂
-        simp at h₂
-        subst h₂
-        exfalso
-        apply h
-        exists y
-      · intros _ _
-        simp
-
-noncomputable def lift_flat (α : Type u) : Dcpo (WithBot α) := @Dcpo.lift _ (Dcpo.flat α)
-
-instance prod : Dcpo (α × β) where
-  sSup := λ s hs => ⟨
-    iSupMem s Prod.fst (Directed.prod_fst hs),
-    iSupMem s Prod.snd (Directed.prod_snd hs)⟩
-  sSup_is_lub := by
-    intros s _
-    constructor
-    · intro ⟨x, y⟩ _
-      constructor <;> apply Dcpo.le_iSupMem <;> assumption
-    · intro ⟨x, y⟩ h
-      constructor <;> apply Dcpo.iSupMem_le <;>
-        intro ⟨x, y⟩ h' <;> cases h h' <;> assumption
-
-theorem prod.sSup {s : Set (α × β)} {hs} :
-  sSup s hs = ⟨iSupMem s Prod.fst (Directed.prod_fst hs), iSupMem s Prod.snd (Directed.prod_snd hs)⟩ := rfl
-
-theorem prod.iSupMem {s : Set ι} {f : ι → α × β} {hf} :
-  iSupMem s f hf = ⟨iSupMem s (Prod.fst ∘ f) (Directed.mono_comp_image hf Monotone.prod_fst), iSupMem s (Prod.snd ∘ f) (Directed.mono_comp_image hf Monotone.prod_snd)⟩ := by
-  trans
-  · apply prod.sSup
-  · congr <;> apply iSupMem.comp
+theorem iSupMem.constant {s : Set ι} {x : α} {hf} :
+  iSupMem s (λ _ => x) hf = x := by
+  apply le_antisymm
+  · apply iSupMem_le; intros _ _; apply le_refl
+  · rcases hf.1 with ⟨_, ⟨i, h₁, h₂⟩⟩
+    subst h₂
+    apply le_iSupMem h₁
 
 theorem sSup_singleton {x : α} :
-  sSup {x} Directed.singleton = x := by
+  sSup {x} Directed'.singleton = x := by
   apply le_antisymm
   · apply sSup_le; simp
   · apply le_sSup; simp
 
 end Dcpo
 
-
-
 structure Continuous [Dcpo α] [Dcpo β] (f : α → β) : Prop where
   mono : Monotone f
-  keeps_sSup : ∀ s hs, f (Dcpo.sSup s hs) = Dcpo.iSupMem s f (Directed.mono_image hs mono)
+  keeps_sSup : ∀ s hs, f (Dcpo.sSup s hs) = Dcpo.iSupMem s f (Directed'.mono_image hs mono)
 
-theorem Continuous.constant [Dcpo α] [Dcpo β] {b} : Continuous (λ _ => b : α → β) where
-  mono := by
-    intros _ _ _; apply le_refl
-  keeps_sSup := by
-    intros s hs
-    apply le_antisymm
-    · apply Dcpo.le_sSup
-      rcases hs.1 with ⟨x, h⟩
-      exists x
-    · apply Dcpo.iSupMem_le
-      intros
-      apply le_refl
+namespace Continuous
 
-def ContinuousDomain (α β) [Dcpo α] [Dcpo β] := { f : α → β // Continuous f }
-infix:min " →ᴰ " => ContinuousDomain
+variable [Dcpo α] [Dcpo β] {f : α → β} (hf : Continuous f)
 
-namespace ContinuousDomain
-
-variable [Dcpo α] [Dcpo β]
-
-instance : CoeFun (α →ᴰ β) (λ _ => α → β) := ⟨Subtype.val⟩
-
-abbrev mono (f : α →ᴰ β) := f.property.mono
-abbrev keeps_sSup (f : α →ᴰ β) := f.property.keeps_sSup
-
-theorem keeps_iSup (f : α →ᴰ β) {g : ι → α} {hg} :
-  f (Dcpo.iSup g hg) = Dcpo.iSup (f ∘ g) (Directed.mono_comp_range hg f.mono) := by
+theorem keeps_iSup {g : ι → α} {hg} :
+  f (Dcpo.iSup g hg) = Dcpo.iSup (f ∘ g) (Directed'.mono_comp_range hg hf.mono) := by
   unfold Dcpo.iSup
-  rw [f.keeps_sSup]
+  rw [hf.keeps_sSup]
   unfold Dcpo.iSupMem
   congr
   ext _
@@ -315,10 +218,10 @@ theorem keeps_iSup (f : α →ᴰ β) {g : ι → α} {hg} :
     exists g i
     aesop
 
-theorem keeps_iSupMem (f : α →ᴰ β) {s : Set ι} {g : ι → α} {hg} :
-  f (Dcpo.iSupMem s g hg) = Dcpo.iSupMem s (f ∘ g) (Directed.mono_comp_image hg f.mono) := by
+theorem keeps_iSupMem {s : Set ι} {g : ι → α} {hg} :
+  f (Dcpo.iSupMem s g hg) = Dcpo.iSupMem s (f ∘ g) (Directed'.mono_comp_image hg hf.mono) := by
   unfold Dcpo.iSupMem
-  rw [f.keeps_sSup]
+  rw [hf.keeps_sSup]
   unfold Dcpo.iSupMem
   congr
   ext _
@@ -331,132 +234,263 @@ theorem keeps_iSupMem (f : α →ᴰ β) {s : Set ι} {g : ι → α} {hg} :
     exists g i
     aesop
 
-end ContinuousDomain
-
-section
-
-variable [Dcpo α] [Dcpo β] [Dcpo γ]
-
-instance : PartialOrder (α →ᴰ β) := by
-  unfold ContinuousDomain
-  exact inferInstance
-
-lemma Monotone.apply {x : α} : Monotone (λ (f : α →ᴰ β) => f x) :=
-  λ _ _ h => h x
-
-lemma Directed.pointwise {s : Set (α →ᴰ β)} (hs : Directed s) :
-  Directed ((λ f => f x) '' s) :=
-  Directed.mono_image hs Monotone.apply
-
-instance Dcpo.continuous : Dcpo (α →ᴰ β) where
-  sSup := λ s hs => ⟨
-    λ x => Dcpo.iSupMem s (λ f => f x) (Directed.pointwise hs),
-    { mono := by
-        intros x y h
-        apply iSupMem_le
-        intros f h₁
-        apply le_trans (f.mono h)
-        apply le_iSupMem h₁
-      keeps_sSup := by
-        intros s' hs'
-        apply le_antisymm
-        · apply iSupMem_le
-          intros f h₁
-          rw [f.keeps_sSup]
-          apply iSupMem_le
-          intros x h₂
-          apply le_trans'
-          · exact le_iSupMem h₂
-          · apply le_iSupMem h₁
-        · apply iSupMem_le
-          intros x h₁
-          apply iSupMem_le
-          intros f h₂
-          apply le_trans'
-          · apply le_iSupMem h₂
-          · apply f.mono
-            exact le_sSup h₁ }⟩
-  sSup_is_lub := by
+theorem constant {b} : Continuous (λ _ => b : α → β) where
+  mono := by
+    intros _ _ _; apply le_refl
+  keeps_sSup := by
     intros s hs
-    constructor
-    · intros f h x
-      apply le_iSupMem h
-    · intros f h x
-      apply iSupMem_le
-      intros g h₁
-      apply h
-      exact h₁
+    apply le_antisymm
+    · apply Dcpo.le_sSup
+      rcases hs.1 with ⟨x, h⟩
+      exists x
+    · apply Dcpo.iSupMem_le
+      intros
+      apply le_refl
 
-theorem Dcpo.continuous.sSup {s : Set (α →ᴰ β)} {hs} :
-  (sSup s hs) x = iSupMem s (λ f => f x) (Directed.pointwise hs) := rfl
+end Continuous
 
-theorem Dcpo.continuous.iSupMem {s : Set ι} {f : ι → (α →ᴰ β)} {hf} :
-  (iSupMem s f hf) x = iSupMem s (λ i => f i x) (Directed.mono_comp_image hf Monotone.apply) := by
+
+
+structure Domain where
+  carrier : Type u
+  dcpo : Dcpo carrier
+  orderBot : OrderBot carrier
+
+instance : CoeSort Domain.{u} (Type u) := ⟨Domain.carrier⟩
+instance {α : Domain} : Dcpo α := α.dcpo
+instance {α : Domain} : OrderBot α := α.orderBot
+
+namespace Domain
+
+def Unit : Domain where
+  carrier := PUnit
+  dcpo := {
+    sSup := λ s _ => ()
+    sSup_is_lub := by
+      intros _ _; constructor <;> intros _ _ <;> trivial
+  }
+  orderBot := inferInstance
+
+def Prod (α β : Domain) : Domain where
+  carrier := α × β
+  dcpo := {
+    sSup := λ s hs => ⟨
+      Dcpo.iSupMem s Prod.fst (Directed'.prod_fst hs),
+      Dcpo.iSupMem s Prod.snd (Directed'.prod_snd hs)⟩
+    sSup_is_lub := by
+      intros s _
+      constructor
+      · intro ⟨x, y⟩ _
+        constructor <;> apply Dcpo.le_iSupMem <;> assumption
+      · intro ⟨x, y⟩ h
+        constructor <;> apply Dcpo.iSupMem_le <;>
+          intro ⟨x, y⟩ h' <;> cases h h' <;> assumption
+  }
+  orderBot := inferInstance
+
+infixr:35 " ×ᴰ " => Prod
+
+theorem Prod.sSup {α β : Domain} {s : Set (α ×ᴰ β)} {hs} :
+  Dcpo.sSup s hs = ⟨
+    Dcpo.iSupMem s Prod.fst (Directed'.prod_fst hs),
+    Dcpo.iSupMem s Prod.snd (Directed'.prod_snd hs)
+  ⟩ := rfl
+
+theorem Prod.iSupMem {s : Set ι} {f : ι → (α ×ᴰ β)} {hf} :
+  Dcpo.iSupMem s f hf = ⟨
+    Dcpo.iSupMem s (Prod.fst ∘ f) (Directed'.mono_comp_image hf Monotone.prod_fst),
+    Dcpo.iSupMem s (Prod.snd ∘ f) (Directed'.mono_comp_image hf Monotone.prod_snd)
+  ⟩ := by
   trans
   · apply sSup
-  · apply iSupMem.comp
+  · congr <;> apply Dcpo.iSupMem.comp
 
+noncomputable def Flat (α : Type u) : Domain :=
+  let instLE : LE (Option α) := {
+    le := λ
+          | some x, some y => x = y
+          | some _, none => False
+          | none, _ => True }
+  { carrier := Option α
+    dcpo := {
+      le_refl := by intro x; cases x <;> simp
+      le_trans := by
+        intros x y z h₁ h₂
+        cases x <;> cases y <;> cases z <;> simp at *
+        simp [h₁, h₂]
+      le_antisymm := by
+        intros x y h _
+        cases x <;> cases y <;> simp at *;
+        simp [h]
+      sSup := λ s _ => have := Classical.propDecidable
+        if h : ∃ x, some x ∈ s then
+          some (Classical.choose h)
+        else none
+      sSup_is_lub := by
+        intros s hs
+        by_cases h : ∃ x, some x ∈ s <;> simp [h]
+        · have hlemma : ∀ x (_ : some x ∈ s)
+            (h' : ∃ x, some x ∈ s), Classical.choose h' = x := by
+            intros x h h'
+            let y := Classical.choose h'
+            rcases hs.2 x h y (Classical.choose_spec h') with ⟨z, _, h₃, h₄⟩
+            cases z <;> simp at *
+            simp [h₃, h₄]
+          constructor
+          · intros x h₁; cases x <;> simp
+            simp [hlemma _ h₁]
+          · intros _ h₁
+            apply h₁
+            apply Classical.choose_spec (p := λ x => some x ∈ s)
+        · constructor
+          · intros x h₁
+            cases x <;> simp
+            exact h ⟨_, h₁⟩
+          · intros _ _; simp
+    }
+    orderBot := {
+      bot := none
+      bot_le := by intro; simp
+    }
+  }
 
+def ContinuousMap (α β : Domain) : Domain where
+  carrier :=
+    { f : α → β // Continuous f }
+  dcpo := {
+    sSup := λ s hs => {
+      val := λ x =>
+        Dcpo.iSupMem s (λ f => f.val x) (by
+          apply Directed'.mono_image hs
+          intros _ _ h
+          apply h)
+      property := {
+        mono := by
+          intros x y h
+          apply Dcpo.iSupMem.mono
+          intros f _
+          exact f.2.mono h
+        keeps_sSup := by
+          intros s' hs'
+          apply le_antisymm
+          · apply Dcpo.iSupMem_le
+            intros f h₁
+            rw [f.2.keeps_sSup]
+            apply Dcpo.iSupMem.mono
+            intros x _
+            apply Dcpo.le_iSupMem h₁
+          · apply Dcpo.iSupMem_le
+            intros x h₁
+            apply Dcpo.iSupMem_le
+            intros f h₂
+            apply le_trans'
+            · apply Dcpo.le_iSupMem h₂
+            · apply f.2.mono
+              exact Dcpo.le_sSup h₁
+        }
+      }
+    sSup_is_lub := by
+      intros s hs
+      constructor
+      · intros f h x
+        apply Dcpo.le_iSupMem h
+      · intros f h x
+        apply Dcpo.iSupMem_le
+        intros g h₁
+        apply h
+        exact h₁
+  }
+  orderBot := {
+    bot := {
+      val := λ _ => ⊥
+      property := Continuous.constant
+    }
+    bot_le := by intro _ _; apply bot_le
+  }
+infixr:25 " →ᴰ " => ContinuousMap
+instance : CoeFun (α →ᴰ β) (λ _ => α → β) :=
+  ⟨Subtype.val⟩
 
-def fst : α × β →ᴰ α where
+theorem ContinuousMap.bot_iff {f : α →ᴰ β} :
+  f = ⊥ ↔ ∀ x, f x = ⊥ := by
+  constructor
+  · intro h; subst h; aesop
+  · intro h; cases f; congr; funext; apply h
+
+lemma _root_.Monotone.apply :
+  Monotone (λ (f : α →ᴰ β) => f x) := by
+  intros _ _ h; simp; apply h
+
+lemma _root_.Directed'.pointwise {s : Set (α →ᴰ β)}
+  (hs : Directed' s) : Directed' ((λ f => f x) '' s) :=
+  Directed'.mono_image hs Monotone.apply
+
+theorem ContinuousMap.sSup {s : Set (α →ᴰ β)} {hs} :
+  (Dcpo.sSup s hs) x = Dcpo.iSupMem s (λ f => f x) (Directed'.pointwise hs) := rfl
+
+theorem ContinuousMap.iSupMem {s : Set ι} {f : ι → (α →ᴰ β).carrier} {hf} :
+  (Dcpo.iSupMem s f hf) x = Dcpo.iSupMem s (λ i => f i x) (Directed'.mono_comp_image hf Monotone.apply) := by
+  trans
+  · apply sSup
+  · apply Dcpo.iSupMem.comp
+
+def fst : α ×ᴰ β →ᴰ α where
   val := Prod.fst
   property := {
     mono := λ _ _ ⟨h, _⟩ => h
     keeps_sSup := λ _ _ => rfl
   }
 
-def snd : α × β →ᴰ β where
+def snd : α ×ᴰ β →ᴰ β where
   val := Prod.snd
   property := {
     mono := λ _ _ ⟨_, h⟩ => h
     keeps_sSup := λ _ _ => rfl
   }
 
-def apply : (α →ᴰ β) × α →ᴰ β where
+def apply : (α →ᴰ β) ×ᴰ α →ᴰ β where
   val := λ ⟨f, x⟩ => f x
   property := {
     mono := by
       intro ⟨f, x⟩ ⟨g, y⟩ ⟨h₁, h₂⟩
       simp at *
       apply le_trans
-      · apply f.mono; exact h₂
+      · apply f.2.mono; exact h₂
       · apply h₁
     keeps_sSup := by
       intros s hs
-      simp [Dcpo.continuous.iSupMem, Dcpo.prod.iSupMem]
+      simp [Prod.sSup, ContinuousMap.iSupMem]
       apply le_antisymm
       · apply Dcpo.iSupMem_le
         intro ⟨f, x⟩ h₁
         simp
-        rw [f.keeps_iSupMem]
+        rw [f.2.keeps_iSupMem]
         apply Dcpo.iSupMem_le
         intro ⟨g, y⟩ h₂
         rcases hs.2 _ h₁ _ h₂ with ⟨⟨h, z⟩, h₃, h₄, h₅⟩
         simp at *
-        apply le_trans (f.mono h₅.2)
+        apply le_trans (f.2.mono h₅.2)
         apply le_trans (h₄.1 z)
         exact Dcpo.le_iSupMem (f := λ ⟨f, x⟩ => f x) h₃
-      · apply Dcpo.iSupMem_le
-        intro ⟨f, x⟩ h₁
-        apply le_trans'
-        · apply Dcpo.le_iSupMem h₁
-        · apply f.mono
-          apply Dcpo.le_iSupMem h₁
+      · apply Dcpo.iSupMem.mono
+        intro ⟨f, x⟩ h
+        apply f.2.mono
+        exact Dcpo.le_iSupMem (f := Prod.snd) h
   }
 
-def curry (f : α × β →ᴰ γ) : (α →ᴰ (β →ᴰ γ)) where
+def curry (f : α ×ᴰ β →ᴰ γ) : (α →ᴰ β →ᴰ γ) where
   val := λ x => {
     val := λ y => f ⟨x, y⟩
     property := {
       mono := by
         intros y₁ y₂ h
-        apply f.mono
+        apply f.2.mono
         exact ⟨le_refl _, h⟩
       keeps_sSup := by
         intros s hs
-        trans f (Dcpo.iSupMem s (λ y => ⟨x, y⟩) (Directed.mono_image hs (λ _ _ => And.intro (le_refl _))))
+        trans f (Dcpo.iSupMem s (λ y => ⟨x, y⟩) (Directed'.mono_image hs (λ _ _ => And.intro (le_refl _))))
         · apply congr_arg
-          rw [Dcpo.prod.iSupMem]
+          rw [Prod.iSupMem]
           congr
           · unfold Dcpo.iSupMem
             conv => lhs; rw [←Dcpo.sSup_singleton (x := x)]
@@ -468,22 +502,22 @@ def curry (f : α × β →ᴰ γ) : (α →ᴰ (β →ᴰ γ)) where
             · aesop
           · ext _
             aesop
-        · rw [f.keeps_iSupMem]
+        · rw [f.2.keeps_iSupMem]
           rfl
     }
   }
   property := {
     mono := by
       intro x₁ x₂ h y
-      apply f.mono
+      apply f.2.mono
       exact ⟨h, le_refl _⟩
     keeps_sSup := by
       intros s hs
       congr
       funext y
-      trans f (Dcpo.iSupMem s (λ x => ⟨x, y⟩) (Directed.mono_image hs (λ _ _ => (And.intro . (le_refl _)))))
+      trans f (Dcpo.iSupMem s (λ x => ⟨x, y⟩) (Directed'.mono_image hs (λ _ _ => (And.intro . (le_refl _)))))
       · apply congr_arg
-        rw [Dcpo.prod.iSupMem]
+        rw [Prod.iSupMem]
         congr
         · ext _
           aesop
@@ -495,7 +529,7 @@ def curry (f : α × β →ᴰ γ) : (α →ᴰ (β →ᴰ γ)) where
           · rcases hs.1 with ⟨y, h⟩
             aesop
           · aesop
-      · rw [f.keeps_iSupMem]
+      · rw [f.2.keeps_iSupMem]
         unfold Dcpo.iSupMem
         congr
         ext _
@@ -510,69 +544,93 @@ def curry (f : α × β →ᴰ γ) : (α →ᴰ (β →ᴰ γ)) where
           exists x
   }
 
-def uncurry (f : α →ᴰ (β →ᴰ γ)) : α × β →ᴰ γ where
+def uncurry (f : α →ᴰ (β →ᴰ γ)) : α ×ᴰ β →ᴰ γ where
   val := λ ⟨x, y⟩ => f x y
   property := {
     mono := by
       intro ⟨x₁, y₁⟩ ⟨x₂, y₂⟩ ⟨h₁, h₂⟩
       simp at *
       trans
-      · exact (f x₁).mono h₂
-      · apply f.mono h₁
+      · exact (f x₁).2.mono h₂
+      · apply f.2.mono h₁
     keeps_sSup := by
       intros s hs
-      simp [f.keeps_iSupMem, Dcpo.continuous.iSupMem]
+      simp [f.2.keeps_iSupMem, Prod.sSup, ContinuousMap.iSupMem]
       apply le_antisymm
       · apply Dcpo.iSupMem_le
         intro ⟨x₁, y₁⟩ h₁
-        rw [(f x₁).keeps_iSupMem]
+        rw [(f x₁).2.keeps_iSupMem]
         apply Dcpo.iSupMem_le
         intro ⟨x₂, y₂⟩ h₂
         rcases hs.2 _ h₁ _ h₂ with ⟨⟨x₃, y₃⟩, h₃, h₄, h₅⟩
-        apply le_trans (f.mono h₄.1 _)
-        apply le_trans ((f x₃).mono h₅.2)
+        apply le_trans (f.2.mono h₄.1 _)
+        apply le_trans ((f x₃).2.mono h₅.2)
         exact Dcpo.le_iSupMem (f := λ ⟨x, y⟩ => f x y) h₃
-      · apply Dcpo.iSupMem_le
+      · apply Dcpo.iSupMem.mono
         intro ⟨x, y⟩ h
-        apply le_trans' (Dcpo.le_iSupMem h)
-        apply (f x).mono
-        exact Dcpo.le_iSupMem h
+        apply (f x).2.mono
+        exact Dcpo.le_iSupMem (f := Prod.snd) h
   }
 
-end
+def constant {α β : Domain} (b : β) : α →ᴰ β :=
+  ⟨λ _ => b, Continuous.constant⟩
 
+def identity : α →ᴰ α  where
+  val := λ x => x
+  property := {
+    mono := by intros _ _ h; exact h
+    keeps_sSup := by intros s hs; simp [Dcpo.iSupMem]
+  }
 
+def comp (f : α →ᴰ β) (g : β →ᴰ γ) : α →ᴰ γ where
+  val := λ x => g (f x)
+  property := {
+    mono := by
+      intros _ _ h
+      apply g.2.mono
+      apply f.2.mono
+      exact h
+    keeps_sSup := by
+      intros s hs
+      simp [f.2.keeps_sSup, g.2.keeps_iSupMem]
+      rfl
+  }
 
-class DcpoBot (α : Type u) extends Dcpo α, OrderBot α
+def fusion (f : α →ᴰ β →ᴰ γ) (g : α →ᴰ β) : α →ᴰ γ where
+  val := λ x => f x (g x)
+  property := {
+    mono := by
+      intros x y h
+      trans
+      · apply f.2.mono h
+      · apply (f y).2.mono; exact g.2.mono h
+    keeps_sSup := by
+      intros s hs
+      simp [f.2.keeps_sSup, g.2.keeps_sSup, ContinuousMap.iSupMem]
+      trans Dcpo.iSupMem s
+        (λ x => Dcpo.iSupMem s (λ y => f x (g y))
+          (Directed'.mono_image hs (λ _ _ h => (f x).2.mono (g.2.mono h))))
+        (Directed'.mono_image hs (λ _ _ h => Dcpo.iSupMem.mono
+          (λ _ _ => f.2.mono h _)))
+      · congr; funext x; apply (f x).2.keeps_iSupMem
+      · apply le_antisymm
+        · apply Dcpo.iSupMem_le
+          intros x h₁
+          apply Dcpo.iSupMem_le
+          intros y h₂
+          rcases hs.2 _ h₁ _ h₂ with ⟨z, h₃, h₄, h₅⟩
+          apply le_trans (f.2.mono h₄ _)
+          apply le_trans ((f z).2.mono (g.2.mono h₅))
+          apply Dcpo.le_iSupMem h₃
+        · apply Dcpo.iSupMem_le
+          intros x h₁
+          apply le_trans' (Dcpo.le_iSupMem h₁)
+          exact Dcpo.le_iSupMem (f := λ y => f x (g y)) h₁
+  }
 
-noncomputable instance [Dcpo α] : DcpoBot (WithBot α) where
-noncomputable def DcpoBot.lift_flat (α : Type u) : DcpoBot (WithBot α) :=
-  @DcpoBot.mk _ (Dcpo.lift_flat α) inferInstance
-
-instance : DcpoBot PUnit where
-instance [DcpoBot α] [DcpoBot β] : DcpoBot (α × β) where
-
-instance DcpoBot.continuous [Dcpo α] [DcpoBot β] : DcpoBot (α →ᴰ β) where
-  bot := ⟨λ _ => ⊥, Continuous.constant⟩
-  bot_le := by intro f x; apply bot_le
-
-namespace ContinuousDomain
-
-theorem bot_iff [Dcpo α] [DcpoBot β] {f : α →ᴰ β} :
-  f = ⊥ ↔ ∀ x, f x = ⊥ := by
-  constructor
-  · intro h; subst h; aesop
-  · intro h
-    cases f
-    simp [Bot.bot]
-    congr
-    funext; apply h
-
-variable [DcpoBot α] (f : α →ᴰ α)
-
-def iter : Nat → α
+def iter (f : α →ᴰ α) : Nat → α
 | 0 => ⊥
-| n + 1 => f (iter n)
+| n + 1 => f (iter f n)
 
 lemma iter_mono : Monotone (iter f) := by
   intro n m h
@@ -582,15 +640,58 @@ lemma iter_mono : Monotone (iter f) := by
     clear h ih
     induction' m with m ih
     · apply bot_le
-    · apply f.mono
+    · apply f.2.mono
       exact ih
 
-def fix : α :=
-  Dcpo.iSup (iter f) (Directed.mono_range Directed.linear_order_univ (iter_mono f))
+lemma iter_mono' : Monotone (λ (f : α →ᴰ α) => iter f n) := by
+  intros f g h
+  induction' n with n ih
+  · apply le_refl
+  · apply le_trans (f.2.mono ih)
+    apply h
+
+def fix : (α →ᴰ α) →ᴰ α where
+  val := λ f => Dcpo.iSup (iter f) (Directed'.mono_range Directed'.linear_order_univ iter_mono)
+  property := {
+    mono := by
+      intros f g h
+      apply Dcpo.iSup.mono
+      intro n
+      apply iter_mono' h
+    keeps_sSup := by
+      intros s hs
+      apply le_antisymm
+      · apply Dcpo.iSup_le
+        intro n
+        induction' n with n ih
+        · apply bot_le
+        · simp [iter, ContinuousMap.sSup]
+          apply Dcpo.iSupMem_le
+          intro f h₁
+          apply le_trans (f.2.mono ih)
+          rw [f.2.keeps_iSupMem]
+          apply Dcpo.iSupMem_le
+          intro g h₂
+          simp [f.2.keeps_iSup]
+          apply Dcpo.iSup_le
+          intro m
+          rcases hs.2 _ h₁ _ h₂ with ⟨h, h₃, h₄, h₅⟩
+          apply le_trans (h₄ _)
+          apply le_trans (h.2.mono (iter_mono' h₅))
+          apply le_trans' (Dcpo.le_iSupMem h₃)
+          exact Dcpo.le_iSup (i := m + 1) (f := iter h)
+      · apply Dcpo.iSupMem_le
+        intro f h
+        apply Dcpo.iSup_le
+        intro n
+        apply le_trans' (Dcpo.le_iSup (i := n))
+        apply iter_mono'
+        exact Dcpo.le_sSup h
+  }
 
 theorem fix_is_fixpoint : f (fix f) = fix f := by
   unfold fix
-  rw [f.keeps_iSup]
+  rw [f.2.keeps_iSup]
   apply le_antisymm
   · apply Dcpo.iSup_le
     intro n
@@ -613,7 +714,7 @@ theorem fix_is_least_fixpoint : f x = x → fix f ≤ x := by
   · apply bot_le
   · unfold iter
     rw [←h]
-    apply f.mono
+    apply f.2.mono
     exact ih
 
-end ContinuousDomain
+end Domain
